Started work on initial_core with memories

concurrency/Asm_core.v
@@ -1,5 +1,5 @@
 Require Import sepcomp.semantics.
-Require Import sepcomp.simulations.
+(* Require Import sepcomp.simulations. *)
 Require Import ZArith List.
 Import ListNotations.
 (*Require Import veric.base. *)
@@ -7,7 +7,7 @@ Require Import compcert.common.Globalenvs.
 Require Import compcert.common.Memory.
 Require Import compcert.lib.Integers.
 Require Import compcert.common.Events.
-Require Import ccc26x86.Asm.
+Require Import compcert.ia32.Asm.
 Require Import Values.
 Import AST.
 
@@ -20,61 +20,34 @@ Definition cl_halted (c: regset) : option val := None.
 
 Definition empty_function : function := 
   mkfunction (mksignature nil None cc_default) nil.
+Check Locations.Outgoing.
 
-
-Definition cl_initial_core (ge: genv) (v: val) (args: list val) : option regset :=
-  match v with
-    Vptr b i =>
-    if Int.eq_dec i Int.zero then
-      match Genv.find_funct_ptr ge b with
-        Some f =>
-  None (* This is wrong. *)
-(*
-        Some (CC_core_State empty_function 
-                    (Scall None
-                                 (Etempvar 1%positive (type_of_fundef f))
-                                 (map (fun x => Etempvar (fst x) (snd x))
-                                      (params_of_types 2%positive
-                                                       (params_of_fundef f))))
-                     (Kseq (Sloop Sskip Sskip) Kstop)
-             empty_env
-             (temp_bindings 1%positive (v::args)))
-*)
-      | _ => None end
-    else None
-  | _ => None
-  end.
-
-Parameter need_a_genv: genv.
-Parameter need_a_mem: mem.
-
-
-Definition get_extcall_arg (rs: regset) (m: mem) (l: Locations.loc) : option val :=
+Definition get_extcall_arg (inout: Locations.slot) (rs: regset) (m: mem) (l: Locations.loc) : option val :=
  match l with
   | Locations.R r => Some (rs (preg_of r))
-  | Locations.S Outgoing ofs ty => 
+  | Locations.S inout ofs ty => 
       let bofs := (Stacklayout.fe_ofs_arg + 4 * ofs)%Z  in
       Mem.loadv (chunk_of_type ty) m
                 (Val.add (rs (IR ESP)) (Vint (Int.repr bofs)))
   end.
 
 Fixpoint get_extcall_arguments
-    (rs: regset) (m: mem) (al: list (rpair Locations.loc)) : option (list val) :=
+    (inout: Locations.slot) (rs: regset) (m: mem) (al: list (rpair Locations.loc)) : option (list val) :=
   match al with
   | One l :: al' => 
-     match get_extcall_arg rs m l with
-     | Some v => match get_extcall_arguments rs m al' with
+     match get_extcall_arg inout rs m l with
+     | Some v => match get_extcall_arguments inout rs m al' with
                          | Some vl => Some (v::vl)
                          | None => None
                         end
      | None => None
     end
   | Twolong hi lo :: al' =>
-     match get_extcall_arg rs m hi with
+     match get_extcall_arg inout rs m hi with
      | Some vhi => 
-       match get_extcall_arg rs m lo with
+       match get_extcall_arg inout rs m lo with
        | Some vlo => 
-        match get_extcall_arguments rs m al' with
+        match get_extcall_arguments inout rs m al' with
                          | Some vl => Some (Val.longofwords vhi vlo :: vl)
                          | None => None
         end
@@ -85,13 +58,53 @@ Fixpoint get_extcall_arguments
   | nil => Some nil
  end.
 
-Definition cl_at_external (rs: regset) : option (external_function * list val) :=
+Definition funsig (fd: Asm.fundef) :=
+  match fd with
+  | Internal f => fn_sig f
+  | External ef => ef_sig ef
+  end.
+
+Fixpoint store_arguments (tys: list typ) (args: list val) (loc: val) (m: mem): option mem :=
+ match tys, args with
+ | Tlong::tys', a::args' => None
+ | ty::tys', a::args' =>
+    match Mem.storev (chunk_of_type ty) m loc a with
+    | Some m' => store_arguments tys' args' (Val.add loc (Vint (Int.repr (typesize ty)))) m'
+    | None => None
+    end
+ | nil, nil => Some m
+ | _, _ => None
+ end.
+
+Definition cl_initial_core (ge: genv) (m: mem) (v: val) (args: list val) : option (regset * option mem) :=
+  match v with
+  | Vptr b i =>  if Int.eq_dec i Int.zero then
+    match  Genv.find_funct_ptr ge b with
+    | Some f =>
+       let fsig := funsig f in
+       let (m', stk) := Mem.alloc m 0 (Conventions1.size_arguments fsig) in
+       match store_arguments fsig.(sig_args) args (Vptr stk Int.zero) m with
+        | Some m'' => 
+           Some ( (Pregmap.init Vundef)
+                      # PC <- v
+                      # ESP <- (Vptr stk Int.zero)
+                      # RA <- Vzero,
+                      Some m'')
+        | _ => None
+       end
+     | _ => None
+   end else None
+   | _ => None
+  end.
+
+
+Definition cl_at_external  (ge: genv) (rs: regset) (m: mem) : option (external_function * list val) :=
   match rs PC with
 (*  | CC_core_Callstate (External ef _ _ _) args _ => Some (ef, args)*)
   | Vptr b i => if Int.eq_dec i Int.zero then
-    match  Genv.find_funct_ptr need_a_genv b with
+    match  Genv.find_funct_ptr ge b with
     | Some (External ef) =>
-     match get_extcall_arguments rs need_a_mem 
+     match get_extcall_arguments Locations.Outgoing rs m
                  (Conventions1.loc_arguments (ef_sig ef)) with
      | Some args => Some (ef, args)
      | None => None
@@ -102,10 +115,10 @@ Definition cl_at_external (rs: regset) : option (external_function * list val) :
   | _ => None
 end.
 
-Definition cl_after_external (vret: option val) (rs: regset) : option regset :=
+Definition cl_after_external  (ge: genv) (vret: option val) (rs: regset) : option regset :=
   match rs PC with
   | Vptr b i => if Int.eq_dec i Int.zero then
-    match  Genv.find_funct_ptr need_a_genv b with
+    match  Genv.find_funct_ptr ge b with
     | Some (External ef) =>
       match vret with
       | Some res => 
@@ -120,12 +133,12 @@ Definition cl_after_external (vret: option val) (rs: regset) : option regset :=
  end.
 
 Definition cl_step ge (q: regset) (m: mem) (q': regset) (m': mem) : Prop :=
-    cl_at_external q = None /\ 
+    cl_at_external ge q m = None /\ 
      Asm.step ge (State q m) Events.E0 (State q' m').
 
 Lemma cl_corestep_not_at_external:
   forall ge m q m' q', 
-          cl_step ge q m q' m' -> cl_at_external q = None.
+          cl_step ge q m q' m' -> cl_at_external ge q m = None.
 Proof.
   intros.
   unfold cl_step in H. destruct H; auto.  
